fe_mul proof done!

Otbn/Examples/FeMul25519.v
@@ -14,6 +14,7 @@ Require Import coqutil.Tactics.Tactics.
 Require Import coqutil.Word.Interface.
 Require Import coqutil.Word.Properties.
 Require Import coqutil.Word.LittleEndianList.
+Require Import coqutil.Z.bitblast.
 Require Import coqutil.Z.PushPullMod.
 Require Import coqutil.Z.ZLib.
 Require Import Otbn.ISA.ISA.
@@ -134,71 +135,433 @@ Section Defs.
 End Defs.
 
 Section Math.
+  Context {word256 : word.word 256} {word256_ok : word.ok word256}.
+
   Local Infix "<<" := Z.shiftl (at level 40) : Z_scope.
   Local Infix ">>" := Z.shiftr (at level 40) : Z_scope.
 
   Definition p : Z := 2^255 - 19.
 
-  Definition to_limb64 (x : Z) : Z * Z * Z * Z :=
-    let x0 := x mod 2^64 in
-    let x1 := (x >> 64) mod 2^64 in
-    let x2 := (x >> 128) mod 2^64 in
-    let x3 := (x >> 192) mod 2^64 in
-    (x0, x1, x2, x3).
+  Lemma all_limbs_eq x :
+    0 <= x < 2^256 ->
+    x = (limb_spec x 0) + (limb_spec x 1) * 2^64 + (limb_spec x 2) * 2^128 + (limb_spec x 3) * 2^192.
+  Proof.
+    cbv [limb_spec]. intros. zsimplify.
+    rewrite <-!Z.land_ones, <-!Z.shiftr_div_pow2, <-!Z.shiftl_mul_pow2 by lia.
+    rewrite <-!Z.or_to_plus by (repeat (rewrite <-?Z.or_to_plus; try solve [Z.bitblast])).
+    Z.bitblast.
+    rewrite !Bool.andb_false_r. cbn [orb].
+    apply Z.testbit_false; [ lia | ].
+    rewrite Z.div_small; [ reflexivity | ].
+    lazymatch goal with |- 0 <= x < 2^?n => assert (2^256 <= 2^n); [ | lia ] end.
+    apply Z.pow_le_mono_r; lia.
+  Qed.
 
+  Section Formula.
+    Context (a b : Z).
+
+    Let a0 := limb_spec a 0.
+    Let a1 := limb_spec a 1.
+    Let a2 := limb_spec a 2.
+    Let a3 := limb_spec a 3.
+    Let b0 := limb_spec b 0.
+    Let b1 := limb_spec b 1.
+    Let b2 := limb_spec b 2.
+    Let b3 := limb_spec b 3.
+    
+    (* high terms *)
+    Definition t :=
+      a0 * b2 + a1 * b1 + a2 * b0 + a3 * b3 * 38
+      + ((a0 * b3 + a1 * b2 + a2 * b1 + a3 * b0) << 64).
+
+    Let t0 := limb_spec t 0.
+    Let t1 := limb_spec t 1.
+    Let t2 := limb_spec t 2.
+    Let t3 := limb_spec t 3.
+
+    Definition high := (t0 << 128) + (t1 << 192).
+    Definition needs_mul38 :=
+      t2 + (t3 << 64) + a1 * b3 + a2 * b2 + a3 * b1 
+      + ((a2 * b3) << 64) + ((a3 * b2) << 64).
+    Local Definition low :=
+      needs_mul38 * 38 + a0 * b0 + ((a0 * b1) << 64) + ((a1 * b0) << 64).
+
+    Definition fe_mul_formula := (low + high) mod p.
+
+    Definition a_limbs := (a0 + a1 * 2^64 + a2 * 2^128 + a3 * 2^192).
+    Lemma a_limbs_eq : 0 <= a < 2^256 -> a = a_limbs.
+    Proof. apply all_limbs_eq. Qed.
+    Definition b_limbs := (b0 + b1 * 2^64 + b2 * 2^128 + b3 * 2^192).
+    Lemma b_limbs_eq : 0 <= b < 2^256 -> b = b_limbs.
+    Proof. apply all_limbs_eq. Qed.
+    Definition t_limbs := (t0 + t1 * 2^64 + t2 * 2^128 + t3 * 2^192).
+    Lemma t_limbs_eq : 0 <= t < 2^256 -> t = t_limbs.
+    Proof. apply all_limbs_eq. Qed.
+
+    Lemma t_formula_correct :
+      0 <= a < 2^256 ->
+      0 <= b < 2^256 ->
+      (a * b) mod p = (a0 * b0 + (a0 * b1 + a1 * b0) * 2^64 + (a1 * b3 + a2 * b2 + a3 * b1) * 38 + (a2 * b3 + a3 * b2) * 2^64 * 38 + t * 2^128) mod p.
+    Proof.
+      intros. rewrite a_limbs_eq, b_limbs_eq by lia.
+      cbv [a_limbs b_limbs t]. rewrite Z.shiftl_mul_pow2 by lia.
+      Z.push_mod. change (38 mod p) with (2^256 mod p). Z.pull_mod.
+      f_equal. lia.
+    Qed.
+    
+    Lemma fe_mul_formula_correct :
+      0 <= a < 2^256 ->
+      0 <= b < 2^256 ->
+      0 <= t < 2^256 ->
+      fe_mul_formula = (a * b) mod p.
+    Proof.
+      intros. rewrite t_formula_correct by lia. rewrite t_limbs_eq by lia.
+      cbv [fe_mul_formula low high needs_mul38 t_limbs].
+      rewrite !Z.shiftl_mul_pow2 by lia.
+      Z.push_mod. change (38 mod p) with (2^256 mod p). Z.pull_mod.
+      f_equal. lia.
+    Qed.
+
+  End Formula.
+  
   (* TODO: derive this part *)
   Definition fe_mul_spec a b : Z :=
-    let '(a0, a1, a2, a3) := to_limb64 a in
-    let '(b0, b1, b2, b3) := to_limb64 b in
-    let hi := mulqacc_spec 0 b3 38 128 in
-    let acc := mulqacc_spec 0 a0 b2 0 in
-    let acc := mulqacc_spec acc a0 b2 0 in
-    let acc := mulqacc_spec acc a1 b1 0 in
-    let acc := mulqacc_spec acc a3 (hi >> 64) 0 in
-    let acc := mulqacc_spec acc a0 b3 64 in
-    let acc := mulqacc_spec acc a1 b2 64 in
-    let acc := mulqacc_spec acc a2 b1 64 in
-    let acc := mulqacc_spec acc a3 b0 64 in
-    let acc := mulqacc_spec acc a3 b0 64 in
-    let hi := so_writeback_spec true hi acc in
+    let a0 := word.wrap (limb_spec a 0) in
+    let a1 := word.wrap (limb_spec a 1) in
+    let a2 := word.wrap (limb_spec a 2) in
+    let a3 := word.wrap (limb_spec a 3) in
+    let b0 := word.wrap (limb_spec b 0) in
+    let b1 := word.wrap (limb_spec b 1) in
+    let b2 := word.wrap (limb_spec b 2) in
+    let b3 := word.wrap (limb_spec b 3) in
+    let hi := word.wrap (mulqacc_spec 0 b3 38 128) in
+    let hi2 := word.wrap (limb_spec hi 2) in
+    let hi3 := word.wrap (limb_spec hi 3) in
+    let acc := word.wrap (mulqacc_spec 0 a0 b2 0) in
+    let acc := word.wrap (mulqacc_spec acc a1 b1 0) in
+    let acc := word.wrap (mulqacc_spec acc a2 b0 0) in
+    let acc := word.wrap (mulqacc_spec acc a3 hi2 0) in
+    let acc := word.wrap (mulqacc_spec acc a0 b3 64) in
+    let acc := word.wrap (mulqacc_spec acc a1 b2 64) in
+    let acc := word.wrap (mulqacc_spec acc a2 b1 64) in
+    let acc := word.wrap (mulqacc_spec acc a3 b0 64) in
+    let acc := word.wrap (mulqacc_spec acc a3 hi3 64) in
+    let hi := word.wrap (so_writeback_spec true hi acc) in
     let acc := acc >> 128 in
-    let hi := addm_spec hi 0 p in
-    let acc := mulqacc_spec acc a1 b3 0 in
-    let acc := mulqacc_spec acc a2 b2 0 in
-    let acc := mulqacc_spec acc a3 b1 0 in
-    let acc := mulqacc_spec acc a2 b3 64 in
-    let acc := mulqacc_spec acc a3 b2 64 in
+    let hi := word.wrap (addm_spec hi 0 p) in
+    let acc := word.wrap (mulqacc_spec acc a1 b3 0) in
+    let acc := word.wrap (mulqacc_spec acc a2 b2 0) in
+    let acc := word.wrap (mulqacc_spec acc a3 b1 0) in
+    let acc := word.wrap (mulqacc_spec acc a2 b3 64) in
+    let acc := word.wrap (mulqacc_spec acc a3 b2 64) in
     let lo := acc in
-    let acc := mulqacc_spec 0 lo 38 0 in
-    let acc := mulqacc_spec acc lo 38 64 in
-    let acc := mulqacc_spec acc lo 38 128 in
-    let acc := mulqacc_spec acc lo 38 192 in
-    let acc := mulqacc_spec acc a0 b0 0 in
-    let acc := mulqacc_spec acc a0 b1 64 in
-    let acc := mulqacc_spec acc a1 b0 64 in
+    let lo0 := word.wrap (limb_spec lo 0) in
+    let lo1 := word.wrap (limb_spec lo 1) in
+    let lo2 := word.wrap (limb_spec lo 2) in
+    let lo3 := word.wrap (limb_spec lo 3) in
+    let acc := word.wrap (mulqacc_spec 0 lo0 38 0) in
+    let acc := word.wrap (mulqacc_spec acc lo1 38 64) in
+    let acc := word.wrap (mulqacc_spec acc lo2 38 128) in
+    let acc := word.wrap (mulqacc_spec acc lo3 38 192) in
+    let acc := word.wrap (mulqacc_spec acc a0 b0 0) in
+    let acc := word.wrap (mulqacc_spec acc a0 b1 64) in
+    let acc := word.wrap (mulqacc_spec acc a1 b0 64) in
     let lo := acc in
-    let r := addm_spec lo hi p in
+    let r := word.wrap (addm_spec lo hi p) in
     r.
 
-  (*
-    let b3_38 := b3 * 38 in
-    let t := a0 * b2 + a1 * b1 + a2 * b0 + a3 * b3_38 in
-    let t := t + ((a0 * b3 + a1 * b2 + a2 * b1 + a3 * b0) << 64) in
-    let '(t0, t1, t2, t3) := to_limb64 t in
-    let high := (t0 + t1 << 64) << 128 in
-    let high := if (p <? high) then (high - p) else high in
-    let low := a1 * b3 + a2 * b2 + a3 * b1 + t2 in
-    let low := low + ((a2 * b3 + a3 * b2 + t3) << 64) in
-    let low := low * 38 in
-    let low := low + (a0 * b0 + ((a0 * b1 + a1 * b0) << 64)) in
-    if (p <? low + high) then low + high - p else low + high.
-   *)
+  Lemma limb_spec_bound v l : 0 <= limb_spec v l < 2^64.
+  Proof. apply Z.mod_pos_bound. lia. Qed.
+
+  Lemma limb3_spec_bound v n :
+    0 <= v < 2^n -> 192 <= n -> 0 <= limb_spec v 3 < 2^(n - 192).
+  Proof.
+    intros. cbv [limb_spec].
+    destr (256 <? n).
+    { pose proof Z.pow_le_mono_r 2 64 (n-192) ltac:(lia) ltac:(lia).
+      lazymatch goal with |- 0 <= ?x mod ?m < _ =>
+                            pose proof Z.mod_pos_bound x m ltac:(lia) end.
+      lia. }
+    { pose proof Z.pow_le_mono_r 2 n 256 ltac:(lia) ltac:(lia).
+      assert (v < 2 ^ (64 * 3) * 2 ^ 64) by (change (2^(64*3) * 2^64) with (2^256); lia).
+      pose proof Z.div_lt_upper_bound v (2^(64 * 3)) (2^64) ltac:(lia) ltac:(lia).
+      pose proof Z.div_pos v (2^(64*3)) ltac:(lia) ltac:(lia).
+      rewrite Z.mod_small by lia.
+      split; [ lia | ]. apply Z.div_lt_upper_bound; [ lia | ].
+      rewrite <-Z.pow_add_r by lia. change (64 * 3) with 192.
+      rewrite Zplus_minus. lia. }
+  Qed.
+
+  Lemma limb_spec_nowrap v l : word.wrap (limb_spec v l) = limb_spec v l.
+  Proof. pose proof limb_spec_bound v l. apply Z.mod_small. lia. Qed.
+
+  (* TODO: move *)
+  Lemma addm_spec_bound x y m :
+    0 <= x < 2^256 ->
+    0 <= y < 2^256 ->
+    0 <= m < 2^256 ->
+    x + y < 2^256 + m ->
+    0 <= addm_spec x y m < 2^256.
+  Proof. cbv [addm_spec]. intros. destruct_one_match; lia. Qed.
+
+  (* TODO: move *)
+  Lemma addm_spec_full_reduce x y m :
+    0 < m -> 0 <= x + y < 2 * m -> addm_spec x y m = (x + y) mod m.
+  Proof.
+    cbv [addm_spec]; intros. destruct_one_match; [ | rewrite Z.mod_small; lia ].
+    rewrite Z.mod_eq by lia.
+    pose proof Z.div_le_lower_bound (x + y) m 1 ltac:(lia) ltac:(lia).
+    pose proof Z.div_lt_upper_bound (x + y) m 2 ltac:(lia) ltac:(lia).
+    replace ((x + y) / m) with 1; lia.
+  Qed.
+
+  Lemma p_bound : 0 < p < 2^255.
+  Proof. vm_compute; split; congruence. Qed.
+
+  Ltac intro_limbs_with_bounds :=
+    repeat
+      lazymatch goal with
+      | |- (let x := limb_spec ?y ?n in _) =>
+          let v := fresh x in
+          intro v;
+          eassert (0 <= v < _) by (first [eapply (limb3_spec_bound y); [ eassumption | .. ]; lia
+                                         | apply limb_spec_bound ])
+      | |- 0 <= ?e /\ _ ?e _ =>
+          lazymatch goal with
+            |- ?G =>
+              let P := (eval pattern e in G) in
+              lazymatch P with
+              | ?P _ =>
+                  lazymatch e with                                
+                  | (let x := limb_spec ?y ?n in ?f) =>
+                      change (let x := limb_spec y n in P f); cbv beta
+                  end
+              end
+          end
+      end.
+
+  Lemma t_bound_exact a b :
+    0 <= a < 2^255 ->
+    0 <= b < 2^255 ->
+    0 <= t a b <= (2^64-1)*(2^64-1)*3 + (2^63-1)*(2^63-1)*38 + 2^64*((2^64-1)*(2^64-1)*2 + (2^64-1)*(2^63-1)*2).
+  Proof.
+    intros. cbv beta delta [t]. intro_limbs_with_bounds.
+    change (255 - 192) with 63 in *.
+    rewrite Z.shiftl_mul_pow2 by lia.
+    split; [ lia |  nia ].
+  Qed.
+
+  Lemma t_bound a b :
+    0 <= a < 2^255 ->
+    0 <= b < 2^255 ->
+    0 <= t a b < 2^194.
+  Proof.
+    split; [ | eapply Z.le_lt_trans ]; [ eapply t_bound_exact; lia .. | ].
+    vm_compute. congruence.
+  Qed.
+
+  Lemma needs_mul38_bound a b :
+    0 <= a < 2^255 ->
+    0 <= b < 2^255 ->
+    0 <= needs_mul38 a b < 2^194.
+  Proof.
+    intros; cbv beta delta [needs_mul38]. pose proof t_bound a b ltac:(lia) ltac:(lia).
+    intro_limbs_with_bounds.
+    rewrite !Z.shiftl_mul_pow2 by lia.
+    split; [ lia | nia ].
+  Qed.
+
+  Lemma low_bound a b :
+    0 <= a < 2^255 ->
+    0 <= b < 2^255 ->
+    0 <= low a b < p.
+  Proof.
+    intros; cbv beta delta [low]. pose proof t_bound a b ltac:(lia) ltac:(lia).
+    intro_limbs_with_bounds.
+    pose proof needs_mul38_bound a b ltac:(lia) ltac:(lia).
+    rewrite !Z.shiftl_mul_pow2 by lia.
+    split; [ lia | cbv [p]; nia ].
+  Qed.
+  
+  Lemma high_bound a b :
+    0 <= a < 2^255 ->
+    0 <= b < 2^255 ->
+    0 <= high a b < 2 * p.
+  Proof.
+    intros; cbv beta delta [high]. pose proof t_bound a b ltac:(lia) ltac:(lia).
+    intro_limbs_with_bounds.
+    rewrite !Z.shiftl_mul_pow2 by lia.
+    split; [ lia | cbv [p]; nia ].
+  Qed.
+
+  Lemma b3_38_bound b :
+    0 <= limb_spec b 3 * 38 < 2^128.
+  Proof.
+    pose proof limb_spec_bound b 3.
+    lia.
+  Qed.
+
+  Lemma b3_38_limbs_eq b :
+    0 <= b < 2^255 ->
+    limb_spec b 3 * 38
+    = ((limb_spec (limb_spec b 3 * 38 * 2 ^ 128) 3) * 2^64)
+      + (limb_spec (limb_spec b 3 * 38 * 2 ^ 128) 2).
+  Proof.
+    cbv [limb_spec]. intros.
+    change (2 ^ (64 * 2)) with (1 * 2^128).
+    change (2 ^ (64 * 3)) with (2^64 * 2^128).
+    rewrite !Z.div_mul_cancel_r by lia. zsimplify.
+    change (2^64 * 2^128) with (2^192).
+    assert (0 <= b / 2^192 < 2^64) by
+      (split; [ apply Z.div_pos | apply Z.div_lt_upper_bound ]; lia).
+    rewrite !(Z.mod_small (_ / _)) by
+      (split; [ apply Z.div_pos | apply Z.div_lt_upper_bound ]; lia).
+    rewrite Z.mod_eq by lia. lia.
+  Qed.
+
+  Lemma high_limbs_eq x :
+    0 <= x < 2^256 ->
+    x >> 128 = (limb_spec x 3) * 2^64 + (limb_spec x 2).
+  Proof.
+    cbv [limb_spec]. intros. rewrite Z.shiftr_div_pow2 by lia.
+    change (2 ^ (64 * 3)) with (2^128 * 2^64).
+    change (2 ^ (64 * 2)) with (2^128).
+    rewrite <-Z.div_div by lia.
+    rewrite (Z.mod_small (_ / _ / _)) by
+      (split; repeat first [ apply Z.div_pos | apply Z.div_lt_upper_bound | lia ]).
+    rewrite Z.mod_eq by lia. lia.
+  Qed.
+
+  Lemma fe_mul_spec_equiv a b :
+    0 <= a < 2^255 ->
+    0 <= b < 2^255 ->
+    fe_mul_spec a b = fe_mul_formula a b.
+  Proof.
+    pose proof p_bound.
+    intros; cbv [fe_mul_formula]. cbv beta delta [fe_mul_spec].
+    rewrite !limb_spec_nowrap.
+    repeat lazymatch goal with
+           | |- (let x := ?y in ?f) = ?g =>
+               change (let x := y in (f = g)); intro
+           end.
+    
+    pose proof t_bound a b ltac:(lia) ltac:(lia).
+
+    (* Find the term that represents t and prove equivalence *)
+    lazymatch goal with
+    | x := context [so_writeback_spec _ _ ?vt] |- _ => assert (vt = t a b)
+    end.
+    { transitivity (t a b mod 2^256); [ | apply Z.mod_small; lia ].
+      subst_lets. cbv [mulqacc_spec word.wrap t]. zsimplify.
+      rewrite !Z.shiftl_mul_pow2 by lia.
+      Z.push_pull_mod.
+      assert (0 <= limb_spec b 3 * 38 * 2^128 < 2^256) by (pose proof b3_38_bound b; nia).
+      rewrite (Z.mod_small (_ * 38 * _)) by lia.
+      etransitivity; [ | rewrite <-(Z.mul_assoc _ (limb_spec b 3) 38);
+                         rewrite b3_38_limbs_eq by lia; reflexivity ].
+      f_equal; lia. }
+
+    pose proof needs_mul38_bound a b ltac:(lia) ltac:(lia).
+ 
+    (* Find the term that represents needs_mul38 * 38 and prove equivalence *)
+    lazymatch goal with
+    | x := context [mulqacc_spec _ ?v 38 192] |- _ =>
+             assert (x = needs_mul38 a b * 38)
+    end.
+    { transitivity ((needs_mul38 a b * 38) mod 2^256); [ | apply Z.mod_small; lia ].
+      (* substitute only the *38 terms *)
+      repeat match goal with
+             | x := word.wrap (mulqacc_spec ?acc ?v 38 ?s) |- _ =>
+                      lazymatch goal with |- context [x] => idtac end;
+                      change_in_goal x (word.wrap (mulqacc_spec acc v 38 s))
+             | x := word.wrap (limb_spec ?v ?n) |- _ =>
+                      lazymatch goal with |- context [x] => idtac end;
+                      change_in_goal x (word.wrap (limb_spec v n))
+             end.
+      rewrite !limb_spec_nowrap.
+      (* find the needs_mul38 subterm *)
+      lazymatch goal with |- context [limb_spec ?v _] => replace v with (needs_mul38 a b) end.
+      2:{ symmetry.
+          transitivity (needs_mul38 a b mod 2^256); [ | apply Z.mod_small; lia ].
+          (* substitute all lets, but use equality for t *)
+          repeat lazymatch goal with
+                 | H : ?x = t a b |- context [?x] => rewrite H
+                 | _ => subst_lets_step
+                 end.
+          cbv [mulqacc_spec word.wrap needs_mul38]. zsimplify.
+          rewrite !Z.shiftl_mul_pow2 by lia.
+          Z.push_pull_mod. rewrite high_limbs_eq by lia.
+          f_equal; lia. }
+      
+      subst_lets. cbv [mulqacc_spec word.wrap t]. zsimplify.
+      rewrite !Z.shiftl_mul_pow2 by lia.
+      Z.push_pull_mod.
+      etransitivity; [ | rewrite (all_limbs_eq (needs_mul38 a b)) by lia; reflexivity ].
+      f_equal; lia. }
+    
+    subst_lets_step.
+    lazymatch goal with
+    | |- word.wrap (addm_spec ?x ?y p) = (low a b + high a b) mod p =>
+        pose proof low_bound a b ltac:(lia) ltac:(lia);
+        pose proof high_bound a b ltac:(lia) ltac:(lia);
+        replace x with (low a b);
+        [ replace y with (addm_spec (high a b) 0 p) | ];
+        [ pose proof Z.mod_pos_bound (high a b) p ltac:(lia);
+          pose proof Z.mod_pos_bound (low a b + high a b) p ltac:(lia);
+          rewrite (addm_spec_full_reduce (high a b)), Z.add_0_r by lia;
+          rewrite addm_spec_full_reduce, Z.add_mod_idemp_r by lia;
+          apply Z.mod_small; lia
+        | symmetry; try subst y
+        | symmetry; try subst x ]
+    end.
+    { (* prove high part equivalence *)
+      lazymatch goal with
+      | |- word.wrap (addm_spec ?x 0 p) = addm_spec (high a b) 0 p =>
+          replace x with (high a b);
+          [ apply Z.mod_small; apply addm_spec_bound; lia | symmetry; try subst x ]
+      end.
+      cbv [so_writeback_spec high].
+      lazymatch goal with
+      | H : ?x = t a b |- context [?x] => rewrite H
+      end.
+      lazymatch goal with
+      | |- context [Z.land ?x (Z.ones 128)] =>
+          replace (Z.land x (Z.ones 128)) with 0
+      end.
+      { zsimplify. cbv [word.wrap limb_spec].
+        rewrite !Z.shiftl_mul_pow2 by lia. zsimplify.
+        change (2^256) with (2^128*2^128). rewrite Z.mul_mod_distr_r by lia.
+        rewrite (Z.rem_mul_r _ (2^64) (2^64)) by lia.
+        lia. }
+      { pose proof b3_38_bound b. subst_lets.
+        rewrite Z.land_ones by lia. cbv [word.wrap mulqacc_spec].
+        rewrite !Z.shiftl_mul_pow2 by lia.
+        rewrite (Z.mod_small _ (2^256)) by lia.
+        zsimplify. Z.push_mod. rewrite Z.mod_same by lia.
+        zsimplify. lia. } }
+
+    transitivity ((low a b) mod 2^256); [ | apply Z.mod_small; lia ].
+    cbv [low].
+    repeat lazymatch goal with
+           | H : ?x = t a b |- context [?x] => rewrite H
+           | H : ?x = needs_mul38 a b * 38 |- context [?x] => rewrite H
+           | _ => subst_lets_step
+           end.
+    cbv [mulqacc_spec word.wrap]. zsimplify.
+    rewrite !Z.shiftl_mul_pow2 by lia.
+    Z.push_pull_mod. f_equal; lia.
+  Qed.
+    
 
   Lemma fe_mul_spec_correct a b :
     0 <= a < 2^255 ->
     0 <= b < 2^255 ->
     fe_mul_spec a b = (a * b) mod p.
-  Admitted.
+  Proof.
+    intros. pose proof t_bound a b ltac:(lia) ltac:(lia).
+    rewrite fe_mul_spec_equiv by lia.
+    apply fe_mul_formula_correct; lia.
+  Qed.
   
 End Math.
 
@@ -212,13 +575,37 @@ Section Proofs.
   Add Ring wring32: (@word.ring_theory 32 word32 word32_ok).
   Add Ring wring256: (@word.ring_theory 256 word256 word256_ok).
 
-  (*
-  (* TODO: move *)
-  Lemma addm_full_reduce x y m :
-    word.unsigned x + word.unsigned y < 2 * m ->
-    word.unsigned (addm_spec x y (word.of_Z m)) = (word.unsigned x + word.unsigned y) mod m.
-  Admitted.
-   *)
+  Lemma limb0_small_constant x : 0 <= x < 2^64 -> limb_spec x 0 = x.
+  Proof. intros; cbv [limb_spec]. zsimplify. apply Z.mod_small; lia. Qed.
+
+
+  Ltac crush_step :=
+    lazymatch goal with
+    | |- word.unsigned (word.of_Z ?x) = word.wrap ?y =>
+        replace y with x; [ solve [apply word.unsigned_of_Z] | ]
+    | |- limb_spec _ ?n = limb_spec _ ?n => f_equal
+    | |- addm_spec _ _ _ = addm_spec _ _ _ => f_equal
+    | |- mulqacc_spec _ _ _ _ = mulqacc_spec _ _ _ _ => f_equal
+    | |- so_writeback_spec _ _ _ = so_writeback_spec _ _ _ => f_equal
+    | |- word.unsigned (word.sru ?x (word.of_Z ?n)) = Z.shiftr ?y ?n =>
+        rewrite word.unsigned_sru_nowrap by (rewrite (word.unsigned_of_Z_nowrap n); lia);
+        rewrite (word.unsigned_of_Z_nowrap n) by lia; f_equal
+    | |- word.unsigned (word.of_Z ?x) = ?x => apply word.unsigned_of_Z_nowrap; lia
+    | |- word.unsigned (word.of_Z (limb_spec (word.unsigned (word.of_Z 38)) 0)) = 38 =>
+        rewrite (word.unsigned_of_Z_nowrap 38) by lia;
+        rewrite (limb0_small_constant 38), (word.unsigned_of_Z_nowrap 38) by lia
+    | |- ?x = ?x => reflexivity
+    end.
+  Ltac subst_next_step :=
+    match goal with
+    | x := ?y |- _ =>
+             lazymatch goal with
+             | |- word.unsigned x = ?rhs => change (word.unsigned y = rhs)
+             | |- ?lhs = x => change (lhs = y)
+             end
+    end.
+  Ltac subst_next := subst_next_step; repeat subst_next_step.
+  Ltac crush := try subst_next; repeat progress (repeat crush_step; subst_next).
 
   Lemma fe_mul_correct regs wregs flags dmem cstack lstack a b :
     (* @param[in]  w22: a, first operand, a < 2^255 *)
@@ -262,31 +649,21 @@ Section Proofs.
     end.
 
     (* helpful assertion *)
-    assert (p < 2^256) by (exact eq_refl).
+    assert (0 <= p < 2^256) by (vm_compute; split; congruence).
 
     (* unfold fe_mul_spec and introduce all its lets *)
     cbv beta delta [fe_mul_spec].
     repeat lazymatch goal with
            | |- ?lhs = (match ?e with pair x y => ?f end) =>
                rewrite (surjective_pairing e); cbn iota;
-               change (let x := fst e in let y := snd e in lhs = f); do 2 intro
+               change (let x := fst e in let y := snd e in lhs = f);
+               let x := fresh in let y := fresh in
+               intros x y; subst x y
            | |- ?lhs = (let x := ?e in ?f) =>
                change (let x := e in lhs = f); intro
            end.
 
-    subst v37.
-    lazymatch goal with
-    | |- word.unsigned (addm_spec ?x ?y (word.of_Z ?m)) = (?a + ?b) mod ?m =>
-        replace a with (word.unsigned x); [ replace b with (word.unsigned y) | ];
-        [ apply addm_full_reduce | .. ]
-    end.
-    {
-      apply addm_full_reduce.
-    rewrite addm_full_reduce.
-    rewrite word.unsigned_of_Z_nowrap by lia.
-    Search addm_spec.
-    
+    crush.    
   Qed.
-
 
 End Proofs.
