Otbn/Util/Tactics/SubstLets.v
@@ -1,6 +1,15 @@
-(* Simple utility tactic that substitutes terms into the goal. *)
+
+(*** Simple utility tactic that substitutes terms into the goal. ***)
+
+Ltac change_in_goal x y :=
+  lazymatch goal with | |- ?G =>
+                          let P := (eval pattern x in G) in
+                          lazymatch P with | ?P _ => change (P y); cbv beta end end.
 Ltac subst_lets_step :=
   multimatch goal with
-  | x := _ |- _ => lazymatch goal with |- context [x] => subst x end
+  | x := ?y |- _ =>
+           lazymatch goal with |- context [x] => idtac end;
+           (* `subst` would inline the let in all the other lets and hypotheses *)
+           change_in_goal x y
   end.
 Ltac subst_lets := repeat subst_lets_step.
